src/safety.lean
@@ -7,12 +7,12 @@ theorem preservation
   : has_typ e' t :=
 begin
   induction stepping generalizing t,
-  apply has_typ.if_ stepping_cond' stepping_yes stepping_no t,
-  exact stepping_ih typ.bool (inversion_if_cond stepping_cond stepping_yes stepping_no t typing),
-  exact inversion_if_yes stepping_cond stepping_yes stepping_no t typing,
-  exact inversion_if_no stepping_cond stepping_yes stepping_no t typing,
-  exact inversion_if_yes exp.true stepping_yes stepping_no t typing,
-  exact inversion_if_no exp.false stepping_yes stepping_no t typing,
+  apply has_typ.if_ stepping_e1' stepping_e2 stepping_e3 t,
+  exact stepping_ih typ.bool (inversion_if_e1 stepping_e1 stepping_e2 stepping_e3 t typing),
+  exact inversion_if_e2 stepping_e1 stepping_e2 stepping_e3 t typing,
+  exact inversion_if_e3 stepping_e1 stepping_e2 stepping_e3 t typing,
+  exact inversion_if_e2 exp.true stepping_e2 stepping_e3 t typing,
+  exact inversion_if_e3 exp.false stepping_e2 stepping_e3 t typing,
 end
 
 theorem progress
@@ -29,14 +29,14 @@ begin
   exact val.false,
   right,
   cases typing_ih_a,
-  cases bool_canonical_forms typing_cond typing_a typing_ih_a,
-  existsi typing_yes,
+  cases bool_canonical_forms typing_e1 typing_a typing_ih_a,
+  existsi typing_e2,
   rewrite h,
-  exact steps.if_yes typing_yes typing_no,
-  existsi typing_no,
+  exact steps.if_e2 typing_e2 typing_e3,
+  existsi typing_e3,
   rewrite h,
-  exact steps.if_no typing_yes typing_no,
+  exact steps.if_e3 typing_e2 typing_e3,
   cases typing_ih_a,
-  existsi (exp.if_ typing_ih_a_w typing_yes typing_no),
-  exact steps.if_cond typing_cond typing_ih_a_w typing_yes typing_no typing_ih_a_h,
+  existsi (exp.if_ typing_ih_a_w typing_e2 typing_e3),
+  exact steps.if_e1 typing_e1 typing_ih_a_w typing_e2 typing_e3 typing_ih_a_h,
 end
